AwsCryptographicMaterialProviders/dafny/AwsCryptographyKeyStoreAdmin/src/MutationStateStructures.dfy
@@ -36,6 +36,9 @@ module {:options "/functionSyntax:4" } MutationStateStructures {
   const AWS_CRYPTO_EC := Structure.AWS_CRYPTO_EC
   const KMS_FIELD := Structure.KMS_FIELD
   const HV_FIELD := Structure.HIERARCHY_VERSION
+  const StringToHierarchyVersion := Structure.StringToHierarchyVersion
+  const HierarchyVersionToString := Structure.HierarchyVersionToString
+
   // Ensures
   // - if KMS ARN, Valid KMS ARN
   // - if EC, Valid non-empty EC, & not restricted field names
@@ -158,7 +161,7 @@ module {:options "/functionSyntax:4" } MutationStateStructures {
     requires MutablePropertiesJson?(deserializedMutableProperties).Pass?
   {
     if |deserializedMutableProperties.obj| == 3
-    then HVUtils.StringToHierarchyVersion(deserializedMutableProperties.obj[2].1.str)
+    then StringToHierarchyVersion(deserializedMutableProperties.obj[2].1.str)
     else KeyStoreTypes.HierarchyVersion.v1
   }
 
@@ -174,7 +177,7 @@ module {:options "/functionSyntax:4" } MutationStateStructures {
     requires MutablePropertiesJson?(deserializedInput).Pass?
   {
     if |deserializedInput.obj| == 3 && deserializedInput.obj[2].0 == HV_FIELD && deserializedInput.obj[2].1.String?
-    then Some(HVUtils.StringToHierarchyVersion(deserializedInput.obj[2].1.str))
+    then Some(StringToHierarchyVersion(deserializedInput.obj[2].1.str))
     else None
   }
 
@@ -259,7 +262,7 @@ module {:options "/functionSyntax:4" } MutationStateStructures {
       else JSONValues.Null;
     var hv: JSONValues.JSON :=
       if Mutations.TerminalHierarchyVersion.Some?
-      then JSONValues.JSON.String(HVUtils.HierarchyVersionToString(Mutations.TerminalHierarchyVersion.value))
+      then JSONValues.JSON.String(HierarchyVersionToString(Mutations.TerminalHierarchyVersion.value))
       else JSONValues.Null;
     // TODO-HV-2-M2 : Ensure that pre-HV-1 Mutation Commitments deserialize
     // such commitments will not have the new HV field
@@ -298,7 +301,7 @@ module {:options "/functionSyntax:4" } MutationStateStructures {
       else None;
     var hv: Option<KeyStoreTypes.HierarchyVersion> :=
       if |MutationsJson.obj| == 3 && MutationsJson.obj[2].1.String?
-      then Some(HVUtils.StringToHierarchyVersion(MutationsJson.obj[2].1.str))
+      then Some(StringToHierarchyVersion(MutationsJson.obj[2].1.str))
       else None;
     var input
       := Types.Mutations(
@@ -352,14 +355,14 @@ module {:options "/functionSyntax:4" } MutationStateStructures {
            [
              (AWS_CRYPTO_EC, EncryptionContextStringToJSON(MutationToApply.Original.customEncryptionContext)),
              (KMS_FIELD, JSONValues.JSON.String(MutationToApply.Original.kmsArn)),
-             (HV_FIELD, JSONValues.JSON.String(HVUtils.HierarchyVersionToString(MutationToApply.Original.hierarchyVersion)))
+             (HV_FIELD, JSONValues.JSON.String(HierarchyVersionToString(MutationToApply.Original.hierarchyVersion)))
            ]);
     var TerminalJson
       := JSONValues.Object(
            [
              (AWS_CRYPTO_EC, EncryptionContextStringToJSON(MutationToApply.Terminal.customEncryptionContext)),
              (KMS_FIELD, JSONValues.JSON.String(MutationToApply.Terminal.kmsArn)),
-             (HV_FIELD, JSONValues.JSON.String(HVUtils.HierarchyVersionToString(MutationToApply.Terminal.hierarchyVersion)))
+             (HV_FIELD, JSONValues.JSON.String(HierarchyVersionToString(MutationToApply.Terminal.hierarchyVersion)))
            ]);
 
     var InputJson := InputMutationsToJson(MutationToApply.Input);
